List Impl 3/?.

Earley_List.thy
@@ -130,6 +130,14 @@ fun \<I>_it :: "nat \<Rightarrow> bins" where
 definition \<II>_it :: "bins" where
   "\<II>_it = \<I>_it (length inp)"
 
+subsection \<open>Wellformed Bins\<close>
+
+definition wf_bin :: "nat \<Rightarrow> bin \<Rightarrow> bool" where
+  "wf_bin k b \<longleftrightarrow> (\<forall>x \<in> set (items b). item_end x = k \<and> wf_item x)"
+
+definition wf_bins :: "bins \<Rightarrow> bool" where
+  "wf_bins bs \<longleftrightarrow> (\<forall>k. wf_bin k (bins bs ! k))"
+
 subsection \<open>Equality of generated bins\<close>
 \<comment>\<open>TODO: distinctness for termination proof\<close>
 
@@ -139,11 +147,59 @@ lemma Init_it_eq_Init:
   by (auto simp: valid_rules; blast)
 
 lemma A:
-  "set_bins bs \<subseteq> I \<Longrightarrow> y \<in> set_bins bs \<Longrightarrow> next_symbol y = None \<Longrightarrow> set (Complete_it k y bs) \<subseteq> Complete k I"
-  sorry
+  assumes "set_bins bs \<subseteq> I" "y \<in> set_bin (bins bs ! k)" "next_symbol y = None" "wf_bins bs" "k < length (bins bs)"
+  shows "set (Complete_it k y bs) \<subseteq> Complete k I"
+proof standard
+  fix x
+  assume *: "x \<in> set (Complete_it k y bs)"
+
+  have "y \<in> set_bins bs"
+    using assms(2) assms(5) nth_mem set_bins_def by auto
+  moreover have "item_end y = k"
+    using assms(2) assms(4) set_bin_def wf_bin_def wf_bins_def by blast
+  ultimately have 0: "y \<in> bin I k"
+    unfolding bin_def using assms(1) by blast
+
+  let ?orig = "bins bs ! item_origin y"
+  let ?xs = "filter (\<lambda>x. next_symbol x = Some (item_rule_head y)) (items ?orig)"
+
+  have "item_origin y < length (bins bs)"
+    by (metis wf_bins_def Orderings.order_class.dual_order.trans assms(2,4,5) less_Suc_eq_le not_less_eq set_bin_def wf_bin_def wf_item_def)
+
+  hence "\<forall>z \<in> set_bin ?orig. z \<in> bin I (item_origin y)"
+    by (smt (verit, best) Union_iff assms(1,4) bin_def mem_Collect_eq nth_mem set_bin_def set_bins_def subset_eq wf_bin_def wf_bins_def)
+
+  hence 2:  "\<forall>z \<in> set ?xs. z \<in> bin I (item_origin y)"
+    by (simp add: set_bin_def)
+
+  then obtain z where 1: "x = inc_item z k" "z \<in> set ?xs"
+    using "*" Complete_it_def by auto
+  hence 3: "next_symbol z = Some (item_rule_head y)"
+    by simp
+  have 4: "z \<in> bin I (item_origin y)"
+    using 1 2 by simp
+  have 5: "is_complete y"
+    using assms(3) next_symbol_def by (metis not_None_eq)
+
+  thm Complete_it_def Complete_def
+
+  show "x \<in> Complete k I"
+    using 0 1(1) 3 4 5 unfolding Complete_def by blast
+qed
+
+lemma B1:
+  "wf_bins bs \<Longrightarrow> \<forall>x \<in> set (Complete_it k y bs). item_end x = k"
+  unfolding wf_bins_def wf_bin_def Complete_it_def inc_item_def by simp
+
+lemma B2:
+  "wf_bins bs \<Longrightarrow> k \<le> length inp \<Longrightarrow> y \<in> set_bin (bins bs ! k) \<Longrightarrow> \<forall>x \<in> set (Complete_it k y bs). wf_item x"
+  unfolding wf_bins_def wf_bin_def wf_item_def Complete_it_def inc_item_def
+  apply (auto)
+   apply (metis Earley_Set.item.sel(1) Option.option.discI is_complete_def item_rule_body_def next_symbol_def not_less_eq_eq)
+  by (metis le_trans set_bin_def)
 
 lemma \<pi>_it'_sub_\<pi>:
-  "set_bins bs \<subseteq> I \<Longrightarrow> set_bins (\<pi>_it' k bs i) \<subseteq> \<pi> k I"
+  "set_bins bs \<subseteq> I \<Longrightarrow> k < length (bins bs) \<Longrightarrow> wf_bins bs \<Longrightarrow> set_bins (\<pi>_it' k bs i) \<subseteq> \<pi> k I"
 proof (induction k bs i arbitrary: I rule: \<pi>_it'.induct)
   case (1 k bs i)
 
@@ -158,27 +214,39 @@ proof (induction k bs i arbitrary: I rule: \<pi>_it'.induct)
   next
     case False
     let ?x = "items (bins bs ! k) ! i"
-    have "?x \<in> set_bin (bins bs ! k)"
+    have 0: "?x \<in> set_bin (bins bs ! k)"
       using False set_bin_def by auto
+    have "?x \<in> set_bins bs"
+      by (smt (verit, del_insts) "local.1.prems"(2) False Union_iff mem_Collect_eq not_le_imp_less nth_mem set_bin_def set_bins_def)
     hence "?x \<in> I"
-      using "1.prems" by (metis Earley_List.bins.collapse Un_iff app_bins_def le_refl list_update_beyond set_bin_def set_bins_app_bins subset_iff)
+      using "1.prems" by (smt (verit, ccfv_SIG) Union_iff in_mono mem_Collect_eq nth_mem set_bins_def)
     show ?thesis
     proof cases
-      assume "next_symbol ?x = None"
+      assume 1: "next_symbol ?x = None"
       have "set_bins (app_bins bs k (Complete_it k ?x bs)) = set_bins bs \<union> set (Complete_it k ?x bs)"
-        by (simp add: set_bins_app_bins)
+        using "1.prems" by (simp add: set_bins_app_bins)
       also have "... \<subseteq> I \<union> set (Complete_it k ?x bs)"
         using "1.prems" by blast
       also have "... \<subseteq> I \<union> Complete k I"
-        using A
-        by (metis "local.1.prems" Earley_List.bins.exhaust_sel False app_bins_def le_cases le_iff_sup list_update_beyond nat_less_le set_bins_app_bins set_update_memI subset_eq sup_commute)
+        using A[OF "1.prems"(1) 0 1] "1.prems"(2,3) by blast
       also have "... = Complete k I"
         using Complete_mono by blast
-      also have "... \<subseteq> \<pi> k I"
-        by (simp add: Complete_\<pi>_mono)
-      finally have "set_bins (app_bins bs k (Complete_it k ?x bs)) \<subseteq> \<pi> k I" .
-      show ?thesis
-        by (metis "1"(2) Earley_List.bins.exhaust_sel False Un_iff \<pi>_mono app_bins_def le_iff_sup linorder_le_cases list_update_beyond nat_less_le set_bins_app_bins set_update_memI subsetI)
+      finally have 0: "set_bins (app_bins bs k (Complete_it k ?x bs)) \<subseteq> Complete k I" .
+
+      have 1: "k < length (bins (app_bins bs k (Complete_it k ?x bs)))"
+        by (simp add: "1.prems"(2) app_bins_def)
+      have 2: "wf_bins (app_bins bs k (Complete_it k (items (bins bs ! k) ! i) bs))"
+        using 0 sledgehammer
+        by (smt (z3) "local.1.prems"(2) "local.1.prems"(3) B2 Earley_List.Earley_List.B1 Earley_List.bins.sel Earley_List_axioms False UnE app_bins_def not_le_imp_less nth_list_update_eq nth_list_update_neq nth_mem set_bin_app_bin set_bin_def wf_bin_def wf_bins_def wf_item_def)
+
+      have "set_bins (\<pi>_it' k bs i) = set_bins (\<pi>_it' k (app_bins bs k (Complete_it k ?x bs)) (i + 1))"
+        by (metis (no_types, lifting) False Option.option.simps(4) \<open>next_symbol (items (bins bs ! k) ! i) = None\<close> local.\<pi>_it'.simps)
+      also have "... \<subseteq> \<pi> k (Complete k I)"
+        using "1.IH"[OF False _ _ 0 1 2] by (simp add: \<open>next_symbol (items (bins bs ! k) ! i) = None\<close>)
+      also have "... \<subseteq> \<pi> k (\<pi> k I)"
+        using Complete_\<pi>_mono by (simp add: \<pi>_sub_mono)
+      finally show ?thesis
+        using \<pi>_idem by blast
     next
       assume "\<not> next_symbol ?x = None"
       show ?thesis
@@ -188,16 +256,54 @@ proof (induction k bs i arbitrary: I rule: \<pi>_it'.induct)
 qed
 
 lemma \<pi>_it_sub_\<pi>:
-  "set_bins bs \<subseteq> I \<Longrightarrow> set_bins (\<pi>_it k bs) \<subseteq> \<pi> k I"
+  "set_bins bs \<subseteq> I \<Longrightarrow> k < length (bins bs) \<Longrightarrow> wf_bins bs \<Longrightarrow> set_bins (\<pi>_it k bs) \<subseteq> \<pi> k I"
   using \<pi>_it'_sub_\<pi> \<pi>_it_def by metis
 
+lemma Q:
+  "wf_bins Init_it"
+  sorry
+
+lemma Q':
+  "wf_bins bs \<Longrightarrow> wf_bins (\<pi>_it k bs)"
+  sorry
+
+lemma Q'':
+  "length (bins (\<pi>_it k bs)) = length (bins bs)"
+  sorry
+
+lemma \<I>_it_length:
+  "length (bins (\<I>_it k)) = length (bins Init_it)"
+  by (induction k) (auto simp: Q'')
+
+lemma \<I>_it_wf_bins:
+  "wf_bins (\<I>_it k)"
+  by (induction k) (auto simp: Q Q')
+
 lemma \<I>_it_sub_\<I>:
-  "set_bins (\<I>_it k) \<subseteq> \<I> k"
-  by (induction k) (auto simp: \<pi>_it_sub_\<pi> Init_it_eq_Init)
+  "k < length (bins Init_it) \<Longrightarrow> set_bins (\<I>_it k) \<subseteq> \<I> k"
+proof (induction k)
+  case 0
+  then show ?case
+    by (auto simp: \<pi>_it_sub_\<pi> Q Init_it_eq_Init)
+next
+  case (Suc k)
+  hence 0: "set_bins (\<I>_it k) \<subseteq> \<I> k"
+    by (simp add: Suc_lessD)
+  have 1: "Suc k < length (bins (\<I>_it k))"
+    using \<I>_it_length local.Suc.prems by force
+  have "set_bins (\<pi>_it (Suc k) (\<I>_it k)) \<subseteq> \<pi> (Suc k) (\<I> k)"
+    using \<pi>_it_sub_\<pi>[OF 0 1] \<I>_it_wf_bins by presburger
+  then show ?case
+    by simp
+qed
+
+lemma Q''':
+  "length (bins Init_it) = length inp + 1"
+  unfolding Init_it_def by simp
 
 lemma \<II>_it_sub_\<II>:
   "set_bins \<II>_it \<subseteq> \<II>"
-  using \<I>_it_sub_\<I> \<II>_def \<II>_it_def by simp
+  using \<I>_it_sub_\<I> \<II>_def \<II>_it_def by (simp add: Q''')
 
 end
 
